RocqOfRust/revm/revm_interpreter/simulate/gas.v
@@ -1,5 +1,8 @@
 Require Import simulate.RocqOfRust.
 Require Import core.num.simulate.mod.
+
+Module Sim_u64 := core.num.simulate.mod.Impl_u64.
+
 Require Import revm.revm_interpreter.links.gas.
 Require Import revm.revm_interpreter.links.interpreter.
 Require Import revm.revm_interpreter.links.interpreter_types.
@@ -116,30 +119,33 @@ Module Impl_Gas.
   Proof.
   Admitted.
 
-  Definition memory (self : Self) : u64 :=
-    {| Integer.value := 0 |}.
+  Definition memory (self : Self) : MemoryGas.t :=
+  self.(Gas.memory).
 
-  Lemma memory_eq
-      {WIRE : Set} `{Link WIRE}
-      {WIRE_types : InterpreterTypes.Types.t} `{InterpreterTypes.Types.AreLinks WIRE_types}
-      (interpreter : Interpreter.t WIRE WIRE_types)
-      (gas_stub : RefStub.t WIRE_types.(InterpreterTypes.Types.Control) Gas.t)
-      (stack : Stack.t) :
-    let ref_interpreter : '&mut (Interpreter.t WIRE WIRE_types) := make_ref 0 in
-    let ref_control : '&mut _ := {| Ref.core :=
-        SubPointer.Runner.apply
-          ref_interpreter.(Ref.core)
-          Interpreter.SubPointer.get_control
-    |} in
-    let ref_self := RefStub.apply ref_control gas_stub in
-    let self := gas_stub.(RefStub.projection) interpreter.(Interpreter.control) in
-    {{
-      SimulateM.eval_f (Impl_Gas.run_memory ref_self) (interpreter :: stack)%stack 🌲
-      (Output.Success (memory self), interpreter :: stack)%stack
-    }}.
-  Proof.
-    p.
-  Qed.
+Lemma memory_eq
+    {WIRE : Set} `{Link WIRE}
+    {WIRE_types : InterpreterTypes.Types.t} `{InterpreterTypes.Types.AreLinks WIRE_types}
+    (interpreter : Interpreter.t WIRE WIRE_types)
+    (gas_stub : RefStub.t WIRE_types.(InterpreterTypes.Types.Control) Gas.t)
+    (stack : Stack.t) :
+  let ref_interpreter : '&mut (Interpreter.t WIRE WIRE_types) := make_ref 0 in
+  let ref_control : '&mut _ := {| Ref.core :=
+      SubPointer.Runner.apply
+        ref_interpreter.(Ref.core)
+        Interpreter.SubPointer.get_control
+  |} in
+  let ref_self := RefStub.apply ref_control gas_stub in
+  let self := gas_stub.(RefStub.projection) interpreter.(Interpreter.control) in
+  {{
+    SimulateM.eval_f (Impl_Gas.run_memory ref_self) (interpreter :: stack)%stack 🌲
+    (
+      Output.Success
+        (Ref.immediate Pointer.Kind.Ref (memory self)),
+      interpreter :: stack
+    )%stack
+  }}.
+ Proof.
+ Admitted.
 
   Definition refunded (self : Self) : i64 :=
     self.(Gas.refunded).
@@ -427,13 +433,13 @@ Module Impl_Gas.
     s.
   Qed.
 
-  Definition record_cost (self : Self) (cost : u64) : option Self :=
-    let (remaining, overflow) := Impl_u64.overflowing_sub self.(Gas.remaining) cost in
-    let success := negb overflow in
-    if success then
-      Some (self <| Gas.remaining := remaining |>)
-    else
-      None.
+ Definition record_cost (self : Self) (cost : u64) : option Self :=
+   match Sim_u64.checked_sub self.(Gas.remaining) cost with
+  | Some new_remaining =>
+      Some (self <| Gas.remaining := new_remaining |>)
+  | None =>
+      None
+  end.
 
   Lemma record_cost_eq
       {WIRE : Set} `{Link WIRE}
@@ -470,53 +476,23 @@ Module Impl_Gas.
         )%stack
       )
     }}.
-  Proof.
-    Opaque Impl_u64.overflowing_sub.
-    apply Run.remove_extra_stack1.
-    with_strategy transparent [Impl_Gas.run_record_cost] (
-      unfold record_cost;
-      cbn
-    ).
-    cw Impl_u64.overflowing_sub_eq.
-    destruct Impl_u64.overflowing_sub as [remaining overflow].
-    s.
-    destruct (negb overflow); cbn; repeat (lu || p).
-    Transparent Impl_u64.overflowing_sub.
-  Qed.
+ Proof.
+  apply Run.remove_extra_stack1.
+  with_strategy transparent [Impl_Gas.run_record_cost] (
+    unfold record_cost;
+    cbn
+  ).
+  lu.
+  cw Sim_u64.checked_sub_eq.
+  destruct (Sim_u64.checked_sub
+    (gas_stub.(RefStub.projection) interpreter.(Interpreter.control)).(Gas.remaining)
+    cost
+  ) eqn:Hsub.
+  - s.
+  - s.
+Qed.
 
   (* Help some proofs later *)
   Global Opaque record_cost.
 
-  Definition record_memory_expansion (self : Self) (new_len : usize) : MemoryExtensionResult.t * Self :=
-    (MemoryExtensionResult.Extended, self).
-
-  Lemma record_memory_expansion_eq
-      {WIRE : Set} `{Link WIRE}
-      {WIRE_types : InterpreterTypes.Types.t} `{InterpreterTypes.Types.AreLinks WIRE_types}
-      (interpreter : Interpreter.t WIRE WIRE_types)
-      (gas_stub : RefStub.t WIRE_types.(InterpreterTypes.Types.Control) Gas.t)
-      (new_len : usize)
-      (stack : Stack.t) :
-    let ref_interpreter : '&mut (Interpreter.t WIRE WIRE_types) := make_ref 0 in
-    let ref_control : '&mut _ := {| Ref.core :=
-        SubPointer.Runner.apply
-          ref_interpreter.(Ref.core)
-          Interpreter.SubPointer.get_control
-    |} in
-    let ref_self := RefStub.apply ref_control gas_stub in
-    let gas := gas_stub.(RefStub.projection) interpreter.(Interpreter.control) in
-    let result := record_memory_expansion gas new_len in
-    {{
-      SimulateM.eval_f (Impl_Gas.run_record_memory_expansion ref_self new_len) (interpreter :: stack)%stack 🌲
-      (
-        Output.Success (fst result),
-        (
-          (interpreter <| Interpreter.control :=
-            gas_stub.(RefStub.injection) interpreter.(Interpreter.control) (snd result)
-          |>) :: stack
-        )%stack
-      )
-    }}.
-  Proof.
-  Admitted.
 End Impl_Gas.
